DecidableAndNP.dfy
@@ -1,0 +1,48 @@
+include "DTM.dfy"
+include "turing_machine.dfy"
+
+ghost predicate isTMADecider (delta:Transitions,inputS:InputSymbols,addTapeS:AdditionalTapeSymbols,q0:State)
+  requires isTapeSymbolsValid(inputS,addTapeS)
+  requires isTransitionsValid(delta,inputS,addTapeS)
+{
+  forall input:seq<string> :: isInputValid(input,inputS) ==> haltsInTM(delta,q0,inputS,addTapeS,input)
+}
+
+
+ghost predicate isLanguageDecidable (lang:Language)
+{
+  exists delta:Transitions,q0:State,inputS:InputSymbols,addTapeS:AdditionalTapeSymbols :: (isTapeSymbolsValid(inputS,addTapeS) 
+  && isTransitionsValid(delta,inputS,addTapeS) 
+  && isTMADecider(delta,inputS,addTapeS,q0) 
+  && (isLanguageAcceptedInTM(delta,inputS,addTapeS,q0,lang) || isLanguageAcceptedInTMInPolynomialTime(delta,inputS,addTapeS,q0,lang))
+  )
+}
+
+
+
+lemma DTMDeciderAlwaysHalts (delta:Transitions,inputS:InputSymbols,addTapeS:AdditionalTapeSymbols,q0:State)
+
+
+ghost predicate isLanguageNPTIME1 (lang:Language)
+{
+  exists delta:Transitions,q0:State,inputS:InputSymbols,addTapeS:AdditionalTapeSymbols :: (isTapeSymbolsValid(inputS,addTapeS) 
+  && isTransitionsValid(delta,inputS,addTapeS) 
+  && isTMADecider(delta,inputS,addTapeS,q0) 
+  && isLanguageAcceptedInTMInPolynomialTime(delta,inputS,addTapeS,q0,lang)
+  && !isTransitionsDeterministic(delta,inputS,addTapeS))
+}
+ghost predicate isLanguageNPTIME2 (lang:Language)
+{
+  exists delta:Transitions,q0:State,inputS:InputSymbols,addTapeS:AdditionalTapeSymbols ::(isTapeSymbolsValid(inputS,addTapeS) 
+  && isTransitionsValid(delta,inputS,addTapeS) 
+  && isTMADecider(delta,inputS,addTapeS,q0) 
+  && isTransitionsDeterministic(delta,inputS,addTapeS)
+  && forall input:seq<string> :: (input in lang) <==> (exists c:seq<string> :: isInputValid(input+c,inputS) && isAcceptedInTMInPolynomialTime(delta,q0,inputS,addTapeS,input+c))
+  )
+}
+lemma NPTIMEisDecidable (lang:Language)
+  requires isLanguageNPTIME1(lang)
+  ensures isLanguageDecidable(lang)
+{
+
+}
